progress on lemma three

Pro4/Correctness.lean
@@ -26,15 +26,33 @@ def primes' (fuel : Nat) : InfiniteList Nat :=
 theorem sieve_correct : ∀ (n m : Nat), ∃ f, (take (primes f) n) = (take (primes' m) n) :=
   by sorry
 
+-- def approx (n : Nat) (s : InfiniteList Nat) : InfiniteList Nat :=
+--   match s with
+--   | .bot => .bot
+--   | .nil => .nil
+--   | .cons x xs =>
+--     match n with
+--     | .zero => .bot
+--     | .succ n =>
+--       .cons x (approx n xs)
+
 def approx (n : Nat) (s : InfiniteList Nat) : InfiniteList Nat :=
-  match s with
-  | .bot => .bot
-  | .nil => .nil
-  | .cons x xs =>
-    match n with
-    | .zero => .bot
-    | .succ n =>
-      .cons x (approx n xs)
+  match n with
+  | .zero => .bot
+  | .succ m =>
+    match s with
+    | .cons x xs => .cons x (approx m xs)
+    | _ => .bot
+    -- | .bot => .bot
+    -- | .nil => .nil
+
+-- def approxWhile (p : Nat → Bool) (s : InfiniteList Nat) : InfiniteList Nat :=
+--   match s with
+--   | .cons x xs =>
+--     if p x
+--       then .cons x (approxWhile p xs)
+--       else .bot
+--   | _ => s
 
 def approxWhile (p : Nat → Bool) (s : InfiniteList Nat) : InfiniteList Nat :=
   match s with
@@ -42,7 +60,7 @@ def approxWhile (p : Nat → Bool) (s : InfiniteList Nat) : InfiniteList Nat :=
     if p x
       then .cons x (approxWhile p xs)
       else .bot
-  | _ => s
+  | _ => .bot
 
 def approxUntil (p : Nat → Bool) (s : InfiniteList Nat) : InfiniteList Nat :=
   match s with
@@ -62,6 +80,8 @@ def geq (idx : Option Nat) : Nat → Bool :=
   | none => λ _ => true
   | some x => λ n => n ≥ x
 
+-- If X < X' and X' is the head of an increasing list L' = X' :: L
+-- then X is not a member of L'
 private theorem not_in_inc (x x' : Nat) (l : InfiniteList Nat) :
   x < x' → increasing (cons x' l) → ¬ mem x (cons x' l) :=
   by
@@ -105,19 +125,51 @@ private theorem not_in_inc (x x' : Nat) (l : InfiniteList Nat) :
 
 private theorem three (n : Nat)
                       (xs : InfiniteList Nat)
-  : (increasing xs) → approx n xs = approxWhile (leq xs n) xs := by
+  : (increasing xs) → (∀ i ≤ n, xs.get (i) ≠ none) →
+    approx (n+1) xs = approxWhile (leq (xs.get (n))) xs := by
 
-    intros inc;
-    revert n
+    intros inc def_to_n;
     induction xs with
-    | bot => simp [approx, approxWhile]
-    | nil => simp [approx, approxWhile]
-    | cons x xs IH =>
-      intro n
-      simp [approx, approxWhile, leq]
-      cases (cons x xs).get n with
-      | none => simp; sorry
-      | some y => sorry
+    | bot => unfold approx; unfold approxWhile; simp
+    | nil => unfold approx; unfold approxWhile; simp
+    | cons a as =>
+      induction n with
+      | zero =>
+        simp; unfold approx; simp_all;
+        unfold approx; unfold approxWhile;
+        have h : leq (InfiniteList.get 0 (cons a as)) a = true := by
+          unfold leq; unfold InfiniteList.get; simp
+        rw [h]; simp; unfold InfiniteList.get; simp;
+        unfold approxWhile;
+        induction as with
+        | cons x' xs' IH =>
+          simp; unfold leq; simp
+          have h1 : ¬ (x' ≤ a) := by
+            unfold increasing at inc; simp; apply inc.left
+          simp [h1]
+        | _ => simp
+
+      -- succ case unfinished
+      | succ m IH =>
+        generalize H : (cons a as).get m = h
+        cases h with
+        | none =>
+          simp at def_to_n; unfold Not at def_to_n;
+          apply def_to_n at H; exfalso; assumption; simp
+        | some x =>
+
+        sorry
+        -- SUCC CASE ATTEMPT:
+        -- simp at IH; unfold approx; unfold approxWhile
+        -- have h0 : InfiniteList.get (m + 1) (cons a as) ≠ none := by
+        --   apply def_to_n; simp
+        -- have h : leq (InfiniteList.get (m + 1) (cons a as)) a := by
+        --   unfold leq
+        --   -- should match with some x
+        --   -- then decide that a <= x bc of inc
+        --   sorry
+        -- rw [h]; simp
+        -- sorry
 
 private theorem four (x : Nat)
                      (xs : InfiniteList Nat)
